Factor out merkle interface

Veritas.Merkle.fst
@@ -5,82 +5,6 @@ open FStar.Classical
 open FStar.Seq
 open Veritas.Memory
 
-(* Nodes in an infinite binary tree *)
-type bin_tree_node = 
-  | Root: bin_tree_node 
-  | LeftChild: n:bin_tree_node -> bin_tree_node
-  | RightChild: n:bin_tree_node -> bin_tree_node
-
-(* Depth of a binary tree node *)
-let rec depth (n:bin_tree_node): Tot nat = 
-  match n with 
-  | Root -> 0
-  | LeftChild n' -> 1 + depth n'
-  | RightChild n' -> 1 + depth n'
-
-(* Parent of a node *)
-let rec parent (n:bin_tree_node{~(Root? n)}): Tot bin_tree_node = 
-  match n with
-  | LeftChild n' -> n'
-  | RightChild n' -> n'
-
-(* Merkle address is simply a bin_tree_node of bounded depth *)
-type merkle_addr = n:bin_tree_node{depth n <= addr_size}
-
-(* Depth of a merkle node *)
-let merkle_depth (a:merkle_addr): Tot (i:nat {i <= addr_size}) = depth a
-
-(* Height of a merkle node *)
-let merkle_height (a:merkle_addr): Tot (i:nat {i <= addr_size}) = addr_size - merkle_depth a
-
-(* Merkle tree root *)
-let merkle_root:merkle_addr = Root
-
-(* Is this a merkle root *)
-let is_merkle_root (a:merkle_addr): Tot bool = (Root? a)
-
-(* Is this a leaf node *)
-let is_merkle_leaf (a:merkle_addr): Tot bool = merkle_height a = 0
-
-(* Helper refinement types of merkle addresses *)
-let merkle_leaf_addr = a:merkle_addr{is_merkle_leaf a}
-let merkle_root_addr = a:merkle_addr{is_merkle_root a}
-let merkle_non_leaf_addr = a:merkle_addr{~(is_merkle_leaf a)}
-let merkle_non_root_addr = a:merkle_addr{~(is_merkle_root a)}
-
-(* Size of a hash value *)
-let hash_size = 256
-
-(* hash_value - bit vector of a specified size *)
-type hash_value = bv_t hash_size
-
-(* value stored at specific nodes of a merkle tree *)
-type merkle_payload = 
-  | MkLeaf: value:payload -> merkle_payload
-  | MkInternal: left:hash_value -> right:hash_value -> merkle_payload
-
-(* merkle payload type conditioned on the address *)
-type merkle_payload_of_addr (a:merkle_addr) = 
-  p:merkle_payload{is_merkle_leaf a && MkLeaf? p || 
-                   not (is_merkle_leaf a) && MkInternal? p}
-
-(* hash function maps a merkle payload to a hash value *)
-assume val hashfn (m:merkle_payload): hash_value
-
-(* Inductive type for hash collisions *) 
-type hash_collision = 
-  | Collision: m1:merkle_payload ->
-               m2:merkle_payload { hashfn m1 == hashfn m2 /\ ~(m1 == m2) } ->
-               hash_collision
-
-(*
- * We want to use Merkle tree ideas to verify memory rw-consistency, where
- * memory is addressed locations of a 256-bit address space. To do that we
- * map (data) addresses to leaf nodes of the merkle tree. The leaf node 
- * for a 256-bit address is obtained by traversing the tree from the root 
- * taking a left child for a 0 bit and right child for a 1 bit
- *)
-
 (* Traverse down a binary tree from a start node (sn) based on a bit vector *)
 let rec traverse_bin_tree (#n:pos) (b:bv_t n) (sn:bin_tree_node): Tot bin_tree_node = 
   if n = 1 
@@ -152,6 +76,8 @@ let rec path_from_root_bv2bin_consistent2 (tn:bin_tree_node{depth tn > 0}):
            append_slices p' (ones_vec #1);
            path_from_root_bv2bin_consistent2 tn'
 
+let hashfn (m:merkle_payload): hash_value = admit()
+
 (* 
  * map each 256 bit address in memory to a leaf node of the 
  * merkle tree
@@ -160,16 +86,7 @@ let addr_to_merkle_leaf (a:addr): Tot merkle_leaf_addr =
   bv_to_bin_tree_node a
 
 (* Inverse of addr_to_merkle_leaf *)
-let merkle_leaf_to_addr (a:merkle_leaf_addr): Tot addr = path_from_root a
+let merkle_leaf_to_addr (ma:merkle_leaf_addr): Tot (a:addr{addr_to_merkle_leaf a = ma}) =
+  path_from_root_bv2bin_consistent2 ma; path_from_root ma
 
-(*
- * merklefn: compute the merkle tree value at each node
- * of the merkle tree
- *)
-let rec merklefn (a:merkle_addr) (mem: memory): Tot (merkle_payload_of_addr a)
-  (decreases (merkle_height a)) = 
-  if is_merkle_leaf a
-  then MkLeaf (mem (path_from_root a))
-  else MkInternal (hashfn (merklefn (LeftChild a) mem))
-                  (hashfn (merklefn (RightChild a) mem))
 
