Veritas.Merkle.fsti
@@ -1,0 +1,96 @@
+module Veritas.Merkle
+
+open FStar.BitVector
+open Veritas.Memory
+
+(* Nodes in an infinite binary tree *)
+type bin_tree_node = 
+  | Root: bin_tree_node 
+  | LeftChild: n:bin_tree_node -> bin_tree_node
+  | RightChild: n:bin_tree_node -> bin_tree_node
+
+(* Depth of a binary tree node *)
+let rec depth (n:bin_tree_node): Tot nat = 
+  match n with 
+  | Root -> 0
+  | LeftChild n' -> 1 + depth n'
+  | RightChild n' -> 1 + depth n'
+
+(* Parent of a node *)
+let rec parent (n:bin_tree_node{~(Root? n)}): Tot bin_tree_node = 
+  match n with
+  | LeftChild n' -> n'
+  | RightChild n' -> n'
+
+(* Merkle address is simply a bin_tree_node of bounded depth *)
+type merkle_addr = n:bin_tree_node{depth n <= addr_size}
+
+(* Depth of a merkle node *)
+let merkle_depth (a:merkle_addr): Tot (i:nat {i <= addr_size}) = depth a
+
+(* Height of a merkle node *)
+let merkle_height (a:merkle_addr): Tot (i:nat {i <= addr_size}) = addr_size - merkle_depth a
+
+(* Merkle tree root *)
+let merkle_root:merkle_addr = Root
+
+(* Is this a merkle root *)
+let is_merkle_root (a:merkle_addr): Tot bool = (Root? a)
+
+(* Is this a leaf node *)
+let is_merkle_leaf (a:merkle_addr): Tot bool = merkle_height a = 0
+
+(* Helper refinement types of merkle addresses *)
+let merkle_leaf_addr = a:merkle_addr{is_merkle_leaf a}
+let merkle_root_addr = a:merkle_addr{is_merkle_root a}
+let merkle_non_leaf_addr = a:merkle_addr{~(is_merkle_leaf a)}
+let merkle_non_root_addr = a:merkle_addr{~(is_merkle_root a)}
+
+(* Size of a hash value *)
+let hash_size = 256
+
+(* hash_value - bit vector of a specified size *)
+type hash_value = bv_t hash_size
+
+(* value stored at specific nodes of a merkle tree *)
+type merkle_payload = 
+  | MkLeaf: value:payload -> merkle_payload
+  | MkInternal: left:hash_value -> right:hash_value -> merkle_payload
+
+(* merkle payload type conditioned on the address *)
+type merkle_payload_of_addr (a:merkle_addr) = 
+  p:merkle_payload{is_merkle_leaf a && MkLeaf? p || 
+                   not (is_merkle_leaf a) && MkInternal? p}
+
+(* hash function maps a merkle payload to a hash value *)
+val hashfn (m:merkle_payload): Tot hash_value
+
+(* Inductive type for hash collisions *) 
+type hash_collision = 
+  | Collision: m1:merkle_payload ->
+               m2:merkle_payload { hashfn m1 == hashfn m2 /\ ~(m1 == m2) } ->
+               hash_collision
+
+(*
+ * We want to use Merkle tree ideas to verify memory rw-consistency, where
+ * memory is addressed locations of a 256-bit address space. To do that we
+ * map (data) addresses to leaf nodes of the merkle tree. The leaf node 
+ * for a 256-bit address is obtained by traversing the tree from the root 
+ * taking a left child for a 0 bit and right child for a 1 bit
+ *)
+
+val addr_to_merkle_leaf (a:addr): Tot merkle_leaf_addr
+
+(* Inverse of addr_to_merkle_leaf *)
+val merkle_leaf_to_addr (ma:merkle_leaf_addr): Tot (a:addr{addr_to_merkle_leaf a = ma})
+
+(*
+ * merklefn: compute the merkle tree value at each node
+ * of the merkle tree
+ *)
+let rec merklefn (a:merkle_addr) (mem: memory): Tot (merkle_payload_of_addr a)
+  (decreases (merkle_height a)) = 
+  if is_merkle_leaf a
+  then MkLeaf (mem (merkle_leaf_to_addr a))
+  else MkInternal (hashfn (merklefn (LeftChild a) mem))
+                  (hashfn (merklefn (RightChild a) mem))
