Makefile
@@ -9,7 +9,7 @@ FLAKY=
 # List the files that should be verified by verify-core and verify-all
 # Those files are the roots from where all dependencies are computed
 FSTAR_FILES := Veritas.SeqAux.fsti Veritas.SeqAux.fst Veritas.Memory.fsti \
-               Veritas.Memory.fst
+               Veritas.Memory.fst Veritas.Merkle.fsti Veritas.Merkle.fst
 
 USE_EXTRACTED_INTERFACES=--use_extracted_interfaces true
 
